Velvet/Core/Testing.lean
@@ -1,0 +1,7 @@
+module
+
+public import Velvet.Core.Testing.Decidable
+public meta import Velvet.Core.Testing.Decidable
+public import Velvet.Core.Testing.Gen
+
+open Velvet.Testing
