Velvet/Examples.lean
@@ -25,3 +25,5 @@ public import Velvet.Examples.LiftingExamples
 public import Velvet.Examples.VelvetAndIntrinsicVerification
 public import Velvet.Examples.SimplestSort
 public import Velvet.Examples.NonDet
+public import Velvet.Examples.Tester
+public meta import Velvet.Examples.Tester
